Define SHA-256
Make it take nums instead of bools to start with.

There is still something wrong with byte order or something here
(comparing against test vectors).

examples/Crypto/SHA-2/sha2Script.sml
@@ -9,22 +9,14 @@ open HolKernel boolLib bossLib Parse
 val _ = new_theory"sha2";
 
 (* TODO: move *)
-Definition bool_to_bit_def:
-  bool_to_bit b = if b then 1 else 0n
-End
-
-val () = cv_auto_trans bool_to_bit_def;
-
-(* TODO: move *)
 val () = cv_auto_trans numposrepTheory.n2l_n2lA;
 
 Definition pad_message_def:
-  pad_message bs =
-  let l = LENGTH bs in
+  pad_message bits =
+  let l = LENGTH bits in
   let n = (l + 1) MOD 512 in
   let k = if n <= 448 then 448 - n else 512 + 448 - n in
   let lb = PAD_LEFT 0 64 $ (if l = 0 then [] else REVERSE $ n2l 2 l) in
-  let bits = MAP bool_to_bit bs in
   bits ++ 1 :: REPLICATE k 0 ++ lb
 End
 
@@ -37,7 +29,6 @@ Proof
   rewrite_tac[pad_message_def, PAD_LEFT, ADD1]
   \\ strip_tac
   \\ BasicProvers.LET_ELIM_TAC
-  \\ rw[Abbr`bits`]
   \\ Cases_on`l = 0` \\ gs[Abbr`n`, Abbr`lb`, Abbr`k`]
   \\ simp[LENGTH_n2l, ADD1, LOG2_def]
   \\ `LOG2 l < 64`
@@ -78,16 +69,16 @@ End
 val () = cv_auto_trans parse_message_def;
 
 Definition initial_hash_value_def:
-  initial_hash_value : word32 list = [
-    0x6a09e667w;
-    0xbb67ae85w;
-    0x3c6ef372w;
-    0xa54ff53aw;
-    0x510e527fw;
-    0x9b05688cw;
-    0x1f83d9abw;
-    0x5be0cd19w
-  ]
+  initial_hash_value = (
+    0x6a09e667w : word32,
+    0xbb67ae85w : word32,
+    0x3c6ef372w : word32,
+    0xa54ff53aw : word32,
+    0x510e527fw : word32,
+    0x9b05688cw : word32,
+    0x1f83d9abw : word32,
+    0x5be0cd19w : word32
+  )
 End
 
 val () = cv_trans_deep_embedding EVAL initial_hash_value_def;
@@ -108,6 +99,17 @@ End
 
 val () = cv_auto_trans sigma0_def;
 val () = cv_auto_trans sigma1_def;
+
+Definition Sigma0_def:
+  Sigma0 (x: word32) = rotr 2 x ?? rotr 13 x ?? rotr 22 x
+End
+
+Definition Sigma1_def:
+  Sigma1 (x: word32) = rotr 6 x ?? rotr 11 x ?? rotr 25 x
+End
+
+val () = cv_auto_trans Sigma0_def;
+val () = cv_auto_trans Sigma1_def;
 
 Definition initial_schedule_loop_def:
   initial_schedule_loop Ws t =
@@ -142,9 +144,109 @@ End
 
 val () = cv_auto_trans initial_schedule_def;
 
-(*
+Definition K_def:
+  K: word32 list = [
+    0x428a2f98w; 0x71374491w; 0xb5c0fbcfw; 0xe9b5dba5w; 0x3956c25bw; 0x59f111f1w; 0x923f82a4w; 0xab1c5ed5w;
+    0xd807aa98w; 0x12835b01w; 0x243185bew; 0x550c7dc3w; 0x72be5d74w; 0x80deb1few; 0x9bdc06a7w; 0xc19bf174w;
+    0xe49b69c1w; 0xefbe4786w; 0x0fc19dc6w; 0x240ca1ccw; 0x2de92c6fw; 0x4a7484aaw; 0x5cb0a9dcw; 0x76f988daw;
+    0x983e5152w; 0xa831c66dw; 0xb00327c8w; 0xbf597fc7w; 0xc6e00bf3w; 0xd5a79147w; 0x06ca6351w; 0x14292967w;
+    0x27b70a85w; 0x2e1b2138w; 0x4d2c6dfcw; 0x53380d13w; 0x650a7354w; 0x766a0abbw; 0x81c2c92ew; 0x92722c85w;
+    0xa2bfe8a1w; 0xa81a664bw; 0xc24b8b70w; 0xc76c51a3w; 0xd192e819w; 0xd6990624w; 0xf40e3585w; 0x106aa070w;
+    0x19a4c116w; 0x1e376c08w; 0x2748774cw; 0x34b0bcb5w; 0x391c0cb3w; 0x4ed8aa4aw; 0x5b9cca4fw; 0x682e6ff3w;
+    0x748f82eew; 0x78a5636fw; 0x84c87814w; 0x8cc70208w; 0x90befffaw; 0xa4506cebw; 0xbef9a3f7w; 0xc67178f2w;
+  ]
+End
+
+val () = cv_trans_deep_embedding EVAL K_def;
+
+Definition Ch_def:
+  Ch (x:word32) y z = (x && y) ?? (¬x && z)
+End
+
+val () = cv_auto_trans Ch_def;
+
+Definition Maj_def:
+  Maj (x:word32) y z = (x && y) ?? (x && z) ?? (y && z)
+End
+
+val () = cv_auto_trans Maj_def;
+
+Definition step3_def:
+  step3 Ws (t, (a, b, c, d, e, f, g, h)) = let
+    t1 = h + Sigma1 e + Ch e f g +
+         if t < 64 then EL t K else 0w +
+         if t < LENGTH Ws then EL t Ws else 0w;
+    t2 = Sigma0 a + Maj a b c;
+    h = g;
+    g = f;
+    f = e;
+    e = d + t1;
+    d = c;
+    c = b;
+    b = a;
+    a = t1 + t2 in
+  (SUC t, (a, b, c, d, e, f, g, h))
+End
+
+val step3_pre_def = cv_auto_trans_pre step3_def;
+
+Theorem step3_pre[cv_pre]:
+  step3_pre Ws v
+Proof
+  rw[step3_pre_def, K_def]
+QED
+
 Definition process_block_def:
-  process_block block
+  process_block hash block = let
+    Ws = initial_schedule block;
+    hs = FUNPOW (step3 Ws) 64 (0, hash);
+  in case (hash, hs) of ((a0,b0,c0,d0,e0,f0,g0,h0),(_,(a,b,c,d,e,f,g,h)))
+  => (a0+a, b0+b, c0+c, d0+d, e0+e, f0+f, g0+g, h0+h)
+End
+
+val () = cv_auto_trans process_block_def;
+
+Definition process_blocks_def:
+  process_blocks bs = FOLDL process_block initial_hash_value bs
+End
+
+val () = cv_auto_trans process_blocks_def;
+
+Definition SHA_256_def:
+  SHA_256 m : 256 word = let
+    p = pad_message m;
+    blocks = parse_message [] p
+  in
+    case process_blocks blocks of
+         (a, b, c, d, e, f, g, h)
+  => concat_word_list [h; g; f; e; d; c; b; a]
+End
+
+val () = cv_auto_trans SHA_256_def;
+
+Definition SHA_256_bytes_def:
+  SHA_256_bytes (bs: word8 list) =
+  SHA_256 $ FLAT $
+    MAP (PAD_RIGHT 0 8 o word_to_bin_list) bs
+End
+
+val () = cv_auto_trans SHA_256_bytes_def;
+
+(*
+cv_eval ``
+  parse_message [] $
+  pad_message $
+  FLAT $ MAP (PAD_RIGHT 0 8 o word_to_bin_list) ([97w; 98w; 99w]: word8 list)
+``
+
+Theorem SHA_256_bytes_abc:
+  SHA_256_bytes (MAP (n2w o ORD) "abc") =
+  0xBA7816BF8F01CFEA414140DE5DAE2223B00361A396177A9CB410FF61F20015ADw
+Proof
+  CONV_TAC(PATH_CONV"lrr"EVAL)
+  \\ (fn g =>
+  top_goal() |> #2 |> lhs |> cv_eval
+  EVAL``ORD #"a"``
 *)
 
 (*
